Demonstrate how to implement an algorithm in OpenSSL

providers/multiplexer/EverCrypt.Specs.fsti
@@ -41,3 +41,6 @@ let sha512_hash_post = fun _ _ _ -> True
 
 let curve_x25519_pre = fun _ -> False
 let curve_x25519_post = fun _ _ _ -> True
+
+let aes256_gcm_encrypt_pre = fun _ -> False
+let aes256_gcm_encrypt_post = fun _ _ _ -> True
