providers/multiplexer/EverCrypt.fsti
@@ -67,3 +67,11 @@ val sha512_hash: dst:uint8_p -> src:uint8_p -> len:uint32_t ->
 
 val x25519: dst:uint8_p -> secret:uint8_p -> base:uint8_p ->
   Stack unit curve_x25519_pre curve_x25519_post
+
+
+/// AES-GCM
+
+val aes256_gcm_encrypt: cipher: uint8_p -> tag:uint8_p -> key:uint8_p ->
+  iv:uint8_p -> plaintext:uint8_p -> len: uint32_t ->
+  ad:uint8_p -> adlen:uint32_t ->
+    Stack unit aes256_gcm_encrypt_pre aes256_gcm_encrypt_post
